cfrontend/IFC.v
@@ -1,0 +1,93 @@
+Require Import Coqlib Errors Maps.
+Require Import Integers Floats Values AST Memory Builtins Events Globalenvs Tags.
+Require Import Ctypes Cop Csyntax Csem.
+Require Import List. Import ListNotations.
+
+Module IFCTags <: Tag.
+  Inductive tag' := H | L | X.
+  Definition tag := tag'.
+
+  Theorem tag_eq_dec : forall t1 t2:tag, {t1 = t2} + {t1 <> t2}.
+  Proof. intros. decide equality. Qed.
+
+  Definition def_tag := X.
+
+  Definition ceil (t1 t2:tag) : tag :=
+    match t1, t2 with
+    | H, _ => H
+    | _, H => H
+    | X, _ => X
+    | _, X => X
+    | L, L => L
+    end.
+  
+  (* Allowed flows:
+    H ~> X
+    L ~> *
+    X ~> *
+   *)
+  Definition may_flow (t1 t2:tag) : bool :=
+    match t1, t2 with
+    | H, L => false
+    | _, _ => true
+    end.
+  
+End IFCTags.
+
+Module IFC : Policy IFCTags.
+  Import IFCTags.
+
+  Definition ltag_smoosh (lts:list tag) :=
+    hd def_tag lts.
+  Fixpoint ltag_unsmoosh (lt: tag) (n:nat) :=
+    match n with
+    | O => []
+    | S n' => lt::(ltag_unsmoosh lt n')
+    end.
+
+  Definition InitPCT := L.
+
+  Variable LocalLow : ident -> bool.
+  Definition VarTag (id:ident) :=
+    if LocalLow id
+    then L
+    else X.
+  
+  Definition ConstT := X.
+
+  (* malloc and free *)
+  Definition LocalAllocT (PCT idt : tag) := Some (PCT, X, idt).
+
+  (* taking addresses *)
+  Definition VarAddrT (PCT pt : tag) := Some (PCT, pt).
+  
+  (* Op flows *)
+  Definition UnopT (PCT vt : tag) :=
+    Some (PCT, ceil PCT vt). (* Question: is PCT ever relevant here? *)
+
+  Definition BinopT (PCT vt1 vt2 : tag) :=
+    Some (PCT, ceil vt1 vt2).
+  
+  (* Loads and Stores *)
+  Definition LoadT (PCT pt vt lt : tag) :=
+    Some (ceil (ceil PCT pt) vt).
+
+  Definition StoreT (PCT pt ovt vt lt : tag) :=
+    match ceil (ceil PCT pt) vt, lt with
+    | H, L => None
+    | s, t => Some (PCT, s, t)
+    end.    
+
+  (* Implicit flows *)
+  Definition IfSplitT (PCT vt : tag) :=
+    Some (ceil PCT vt, PCT).
+
+  Definition IfJoinT (PCT pct : tag) :=
+    Some pct.
+  
+  (* Call and return *)
+
+  (* Dummy *)
+  Definition DummyT (ts:list tag) : option (list tag) := Some [].
+
+End IFC.
