cfrontend/Memsafe.v
@@ -1,0 +1,88 @@
+Require Import Coqlib Errors Maps.
+Require Import Integers Floats Values AST Memory Builtins Events Globalenvs Tags.
+Require Import Ctypes Cop Csyntax Csem.
+Require Import List. Import ListNotations.
+
+Module MemTags <: Tag.
+  Inductive tag' :=
+  | X : tag'
+  | Ptr : nat -> tag'
+  | Mem : nat -> tag'
+  | Next : nat -> tag'
+  .
+  
+  Definition tag := tag'.
+
+  Theorem tag_eq_dec : forall t1 t2:tag, {t1 = t2} + {t1 <> t2}.
+  Proof. intros. repeat (decide equality). Qed.
+
+  Definition def_tag := X.
+
+  Definition ptr_match (pt lt : tag) :=
+    match pt, lt with
+    | Ptr n1, Mem n2 => (n1 =? n2)%nat
+    | _, _ => false
+    end.
+  
+End MemTags.
+
+Module PVI : Policy MemTags.
+  Import MemTags.
+
+  Definition ltag_smoosh (lts:list tag) :=
+    hd def_tag lts.
+  Fixpoint ltag_unsmoosh (lt: tag) (n:nat) :=
+    match n with
+    | O => []
+    | S n' => lt::(ltag_unsmoosh lt n')
+    end.
+
+  Definition InitPCT := Next 0.
+
+  Definition VarTag (id:ident) := X.
+  
+  Definition ConstT := X.
+
+  (* malloc and free *)
+  Definition LocalAllocT (PCT idt : tag) :=
+    match PCT with
+    | Next n => Some (Next (S n), Ptr n, Mem n)
+    | _ => None
+    end.
+
+  (* taking addresses *)
+  Definition VarAddrT (PCT pt : tag) := Some (PCT, pt).
+  
+  
+  Definition UnopT (PCT vt : tag) :=
+    Some (PCT, vt). (* Question: is PCT ever relevant here? *)
+
+  (* Pointer arithmetic *)
+  Definition BinopT (PCT vt1 vt2 : tag) :=
+    match vt1, vt2 with
+    | Ptr n, X => Some (PCT, Ptr n)
+    | X, Ptr n => Some (PCT, Ptr n)
+    | X, X => Some (PCT, X)
+    | _, _ => None
+    end.
+
+  (* Load and Store *)
+  Definition LoadT (PCT pt vt lt : tag) :=
+    if ptr_match pt lt
+    then Some vt
+    else None.
+
+  Definition StoreT (PCT pt ovt vt lt : tag) :=
+    if ptr_match pt lt
+    then Some (PCT, vt, lt)
+    else None.
+
+  Definition IfSplitT (PCT vt : tag) :=
+    Some (PCT, PCT).
+
+  Definition IfJoinT (PCT pct : tag) :=
+    Some PCT.
+  
+  Definition DummyT (ts:list tag) : option (list tag) := Some [].
+
+End PVI.
